Affine/Misc.lean
@@ -1,5 +1,6 @@
 import Mathlib.Data.Nat.Basic
 import Mathlib.Data.Finset.Lattice
+import Mathlib.Data.Finset.Sort
 
 theorem Nat.add_le_one {a b : ℕ} : a + b ≤ 1 → a = 0 ∨ b = 0 := by sorry
 
@@ -8,3 +9,11 @@ def Finset.fresh (s : Finset ℕ) : ℕ :=
     s.max' h + 1
   else
     0
+
+-- instance : ToString (Finset ℕ) := ⟨
+--   let trans : IsTrans String (· < ·) := sorry
+--   let trans : IsAntisymm String (· < ·) := sorry
+--   let trans : IsTotal String (· < ·) := sorry
+
+--   fun finset => ", ".intercalate ((finset.val.map ToString.toString).sort (· < ·))
+-- ⟩
